WIP

Phi_Semantics/PhiSem_Aggregate_Base.thy
@@ -7,13 +7,14 @@ text \<open>The base for aggregate values which have inner structures and whose 
 
 section \<open>Semantics\<close>
 
-type_synonym index = nat
+type_synonym aggregate_index = nat
+type_synonym aggregate_path = \<open>aggregate_index list\<close>
 
 debt_axiomatization
-        valid_idx_step :: \<open>TY \<Rightarrow> index \<Rightarrow> bool\<close>
-    and idx_step_type  :: \<open>index \<Rightarrow> TY \<Rightarrow> TY\<close>
-    and idx_step_value :: \<open>index \<Rightarrow> VAL \<Rightarrow> VAL\<close>
-    and idx_step_mod_value :: \<open>index \<Rightarrow> (VAL \<Rightarrow> VAL) \<Rightarrow> VAL \<Rightarrow> VAL\<close>
+        valid_idx_step :: \<open>TY \<Rightarrow> aggregate_index \<Rightarrow> bool\<close>
+    and idx_step_type  :: \<open>aggregate_index \<Rightarrow> TY \<Rightarrow> TY\<close>
+    and idx_step_value :: \<open>aggregate_index \<Rightarrow> VAL \<Rightarrow> VAL\<close>
+    and idx_step_mod_value :: \<open>aggregate_index \<Rightarrow> (VAL \<Rightarrow> VAL) \<Rightarrow> VAL \<Rightarrow> VAL\<close>
     and type_measure :: \<open>TY \<Rightarrow> nat\<close>
 where idx_step_value_welltyp:
            \<open>valid_idx_step T i
@@ -106,16 +107,16 @@ section \<open>Instructions\<close>
     else Fail)" *)
 
 
-definition op_get_aggregate :: "index list \<Rightarrow> TY \<Rightarrow> (VAL, VAL) proc'"
+definition op_get_aggregate :: "aggregate_path \<Rightarrow> TY \<Rightarrow> (VAL, VAL) proc'"
   where "op_get_aggregate idx T = (\<lambda>v.
     \<phi>M_getV T id v (\<lambda>v'.
     \<phi>M_assert (valid_index T idx) \<ggreater>
     Return (\<phi>arg (index_value idx v'))
 ))"
 
-debt_axiomatization allow_assigning_different_typ :: \<open>TY \<Rightarrow> index list \<Rightarrow> bool\<close>
+debt_axiomatization allow_assigning_different_typ :: \<open>TY \<Rightarrow> aggregate_path \<Rightarrow> bool\<close>
 
-definition op_set_aggregate :: "TY \<Rightarrow> TY \<Rightarrow> index list \<Rightarrow> (VAL \<times> VAL, VAL) proc'"
+definition op_set_aggregate :: "TY \<Rightarrow> TY \<Rightarrow> aggregate_path \<Rightarrow> (VAL \<times> VAL, VAL) proc'"
   where "op_set_aggregate Tt Tv idx = 
     \<phi>M_caseV (\<lambda>v tup.
     \<phi>M_assert (valid_index Tt idx \<and> (index_type idx Tt = Tv \<or> allow_assigning_different_typ Tt idx)) \<ggreater>
@@ -148,10 +149,10 @@ lemmas [eval_semantic_index] = nth_Cons_0 nth_Cons_Suc fold_simps list.size simp
 
 subsection \<open>Index to Fields of Structures\<close>
 
-definition \<phi>Index_getter :: \<open>nat list \<Rightarrow> (VAL,'a) \<phi> \<Rightarrow> (VAL,'b) \<phi> \<Rightarrow> ('a \<Rightarrow> 'b) \<Rightarrow> bool\<close>
+definition \<phi>Index_getter :: \<open>aggregate_path \<Rightarrow> (VAL,'a) \<phi> \<Rightarrow> (VAL,'b) \<phi> \<Rightarrow> ('a \<Rightarrow> 'b) \<Rightarrow> bool\<close>
   where \<open>\<phi>Index_getter idx T U g \<longleftrightarrow> index_value idx \<in> (g \<Ztypecolon> T \<Rrightarrow> U)\<close>
 
-definition \<phi>Index_mapper :: \<open>nat list \<Rightarrow> (VAL,'a) \<phi> \<Rightarrow> (VAL,'a2) \<phi> \<Rightarrow> (VAL,'b) \<phi> \<Rightarrow> (VAL,'b2) \<phi> \<Rightarrow> (('b \<Rightarrow> 'b2) \<Rightarrow> 'a \<Rightarrow> 'a2) \<Rightarrow> bool\<close>
+definition \<phi>Index_mapper :: \<open>aggregate_path \<Rightarrow> (VAL,'a) \<phi> \<Rightarrow> (VAL,'a2) \<phi> \<Rightarrow> (VAL,'b) \<phi> \<Rightarrow> (VAL,'b2) \<phi> \<Rightarrow> (('b \<Rightarrow> 'b2) \<Rightarrow> 'a \<Rightarrow> 'a2) \<Rightarrow> bool\<close>
   where \<open>\<phi>Index_mapper idx T T' U U' f
     \<longleftrightarrow> (\<forall>g g'. g \<in> (g' \<Ztypecolon> U \<Rrightarrow> U') \<longrightarrow> index_mod_value idx g \<in> (f g' \<Ztypecolon> T \<Rrightarrow> T'))\<close>
 
@@ -175,7 +176,7 @@ subsection \<open>IDE-Interfaces\<close>
 
 term ParamTag
 
-definition Index_Param_Tag :: \<open>index list \<Rightarrow> bool\<close> ("\<i>\<n>\<d>\<e>\<x> \<p>\<a>\<r>\<a>\<m> _" [1000] 26)
+definition Index_Param_Tag :: \<open>aggregate_path \<Rightarrow> bool\<close> ("\<i>\<n>\<d>\<e>\<x> \<p>\<a>\<r>\<a>\<m> _" [1000] 26)
   where "\<i>\<n>\<d>\<e>\<x> \<p>\<a>\<r>\<a>\<m> x \<equiv> True"
 
 lemma Index_Param_Tag_Swap:
@@ -183,8 +184,6 @@ lemma Index_Param_Tag_Swap:
   unfolding Index_Param_Tag_def ..
 
 ML_file \<open>syntax/index_param.ML\<close>
-
-ML \<open>Scan.pass\<close>
 
 \<phi>processor set_index_param 5000 (premises \<open>\<i>\<n>\<d>\<e>\<x> \<p>\<a>\<r>\<a>\<m> _\<close>) \<open>fn (ctxt,sequent) =>
   Scan.pass (Context.Proof ctxt) Synt_Index_Param.index_term_parser >> (fn term => fn _ =>
